# Factoring by Grouping

## Introduction

Factoring by grouping is an algebraic method used to solve quadratic equations, especially when they are part of a larger expression or when direct factoring isn’t immediately apparent. This method involves rearranging and grouping the terms of the equation in a way that makes it easier to factor and solve. Here’s a step-by-step tutorial on how to factor quadratics by grouping:

### Step 1: Ensure the Equation is in Standard Form

Make sure the quadratic equation is in the standard form:

$$
ax^2 + bx + c = 0
$$

If it’s not, rearrange the terms to get it into this form.

### Step 2: Multiply *a* and *c*

In the standard form equation, multiply the coefficient $$a$$ (in front of $$x^2$$) by the constant term $$c$$. This step is crucial for finding a pair of numbers that can be used to split the middle term.

### Step 3: Find Two Numbers

You need to find two numbers that multiply together to give the product of $$a \times c$$ and add up to $$b$$ (the coefficient of the $$x$$ term).

### Step 4: Rewrite the Middle Term

Using the two numbers found in Step 3, rewrite the middle term $$bx$$ as two terms that can be grouped. Essentially, you’re breaking down $$bx$$ into two terms whose coefficients sum up to $$b$$.

### Step 5: Group and Factor

1. **Group the Terms:** Divide the quadratic equation into two groups that can each be factored.
2. **Factor Out the Greatest Common Factor (GCF):** For each group, factor out the GCF. Ideally, this step will reveal a common factor in each group.

### Step 6: Factor Out the Common Binomial

Once you’ve grouped the terms and factored out the GCF from each group, you should have a common binomial factor. Factor this binomial out of each group.

### Step 7: Solve for *x*

After factoring, you will have an equation set equal to zero. Set each factor (now in a much simpler form) equal to zero and solve for $$x$$.

## Example:

Solve the quadratic equation $$6x^2 + 5x - 6 = 0$$ by factoring by grouping.

1. **Step 1: Standard Form**  
   The equation is already in standard form.

2. **Step 2: Multiply *a* and *c***  
   $$6 \times (-6) = -36$$

3. **Step 3: Find Two Numbers**  
   We need two numbers that multiply to $$-36$$ and add to $$5$$. These numbers are $$9$$ and $$-4$$, because $$9 \times (-4) = -36$$ and $$9 + (-4) = 5$$.

4. **Step 4: Rewrite the Middle Term**  
   $$6x^2 + 9x - 4x - 6 = 0$$

5. **Step 5: Group and Factor**  
   Group the terms: $$(6x^2 + 9x) - (4x + 6) = 0$$  
   Factor out the GCF from each group: $$3x(2x + 3) - 2(2x + 3) = 0$$

6. **Step 6: Factor Out the Common Binomial**  
   The common binomial factor is $$2x + 3$$:  
   $$(3x - 2)(2x + 3) = 0$$

7. **Step 7: Solve for *x***  
   Set each factor equal to zero:  
   $$3x - 2 = 0$$ leads to $$x = \frac{2}{3}$$  
   $$2x + 3 = 0$$ leads to $$x = -\frac{3}{2}$$

Solutions:  
$$
x = \frac{2}{3} \quad \text{and} \quad x = -\frac{3}{2}
$$

## Practice Problem:

Try solving $$3x^2 + 10x + 3 = 0$$ by factoring by grouping.

Factoring by grouping can initially seem less straightforward for quadratics, as it typically involves an additional step of splitting the middle term. However, it becomes a powerful technique once understood, offering an alternative route to solving quadratic equations, especially when direct factoring isn’t possible.

## Exercises

### Easy

1. Solve the quadratic equation $$2x^2 + 7x + 3 = 0$$ by factoring by grouping.
2. Solve the quadratic equation $$3x^2 + 8x + 4 = 0$$ by factoring by grouping.
3. Solve the quadratic equation $$4x^2 + 11x + 6 = 0$$ by factoring by grouping.
4. Solve the quadratic equation $$5x^2 + 14x + 8 = 0$$ by factoring by grouping.
5. Solve the quadratic equation $$2x^2 + 9x + 4 = 0$$ by factoring by grouping.
6. Solve the quadratic equation $$3x^2 + 10x + 3 = 0$$ by factoring by grouping.

### Medium

7. Solve the quadratic equation $$6x^2 + 13x + 6 = 0$$ by factoring by grouping.
8. Solve the quadratic equation $$4x^2 + 17x + 10 = 0$$ by factoring by grouping.
9. Solve the quadratic equation $$5x^2 + 19x + 12 = 0$$ by factoring by grouping.
10. Solve the quadratic equation $$7x^2 + 22x + 8 = 0$$ by factoring by grouping.
11. Solve the quadratic equation $$8x^2 + 14x + 3 = 0$$ by factoring by grouping.
12. Solve the quadratic equation $$9x^2 + 18x + 4 = 0$$ by factoring by grouping.
13. Solve the quadratic equation $$10x^2 + 23x + 10 = 0$$ by factoring by grouping.
14. Solve the quadratic equation $$6x^2 + 25x + 9 = 0$$ by factoring by grouping.
15. Solve the quadratic equation $$7x^2 + 27x + 12 = 0$$ by factoring by grouping.
16. Solve the quadratic equation $$8x^2 + 26x + 9 = 0$$ by factoring by grouping.
17. Solve the quadratic equation $$4x^2 + 15x + 6 = 0$$ by factoring by grouping.
18. Solve the quadratic equation $$5x^2 + 16x + 3 = 0$$ by factoring by grouping.

### Hard

19. Solve the quadratic equation $$12x^2 + 29x + 10 = 0$$ by factoring by grouping.
20. Solve the quadratic equation $$15x^2 + 34x + 12 = 0$$ by factoring by grouping.
21. Solve the quadratic equation $$20x^2 + 39x + 18 = 0$$ by factoring by grouping.
22. Solve the quadratic equation $$24x^2 + 45x + 18 = 0$$ by factoring by grouping.
23. Solve the quadratic equation $$16x^2 + 41x + 15 = 0$$ by factoring by grouping.
24. Solve the quadratic equation $$14x^2 + 37x + 15 = 0$$ by factoring by grouping.

## Solutions

### Easy

1. **Solve the quadratic equation $$2x^2 + 7x + 3 = 0$$ by factoring by grouping:**  
   **Step 1:** The equation is already in standard form.  
   **Step 2:** Multiply $$a$$ and $$c$$: $$2 \times 3 = 6$$.  
   **Step 3:** Find two numbers that multiply to 6 and add to 7: $$6 \times 1 = 6$$ and $$6 + 1 = 7$$.  
   **Step 4:** Rewrite the middle term: $$2x^2 + 6x + x + 3 = 0$$.  
   **Step 5:** Group and factor: $$(2x^2 + 6x) + (x + 3) = 0$$. Factor out the GCF: $$2x(x + 3) + 1(x + 3) = 0$$.  
   **Step 6:** Factor out the common binomial: $$(2x + 1)(x + 3) = 0$$.  
   **Step 7:** Solve for $$x$$: $$2x + 1 = 0$$ gives $$x = -\frac{1}{2}$$ and $$x + 3 = 0$$ gives $$x = -3$$.  
   Solutions:  
   $$
   x = -\frac{1}{2}, \quad x = -3
   $$

3. **Solve the quadratic equation $$4x^2 + 11x + 6 = 0$$ by factoring by grouping:**  
   **Step 1:** The equation is already in standard form.  
   **Step 2:** Multiply $$a$$ and $$c$$: $$4 \times 6 = 24$$.  
   **Step 3:** Find two numbers that multiply to 24 and add to 11: $$8 \times 3 = 24$$ and $$8 + 3 = 11$$.  
   **Step 4:** Rewrite the middle term: $$4x^2 + 8x + 3x + 6 = 0$$.  
   **Step 5:** Group and factor: $$(4x^2 + 8x) + (3x + 6) = 0$$. Factor out the GCF: $$4x(x + 2) + 3(x + 2) = 0$$.  
   **Step 6:** Factor out the common binomial: $$(4x + 3)(x + 2) = 0$$.  
   **Step 7:** Solve for $$x$$: $$4x + 3 = 0$$ gives $$x = -\frac{3}{4}$$ and $$x + 2 = 0$$ gives $$x = -2$$.  
   Solutions:  
   $$
   x = -\frac{3}{4}, \quad x = -2
   $$

5. **Solve the quadratic equation $$2x^2 + 9x + 4 = 0$$ by factoring by grouping:**  
   **Step 1:** The equation is already in standard form.  
   **Step 2:** Multiply $$a$$ and $$c$$: $$2 \times 4 = 8$$.  
   **Step 3:** Find two numbers that multiply to 8 and add to 9: $$8 \times 1 = 8$$ and $$8 + 1 = 9$$.  
   **Step 4:** Rewrite the middle term: $$2x^2 + 8x + x + 4 = 0$$.  
   **Step 5:** Group and factor: $$(2x^2 + 8x) + (x + 4) = 0$$. Factor out the GCF: $$2x(x + 4) + 1(x + 4) = 0$$.  
   **Step 6:** Factor out the common binomial: $$(2x + 1)(x + 4) = 0$$.  
   **Step 7:** Solve for $$x$$: $$2x + 1 = 0$$ gives $$x = -\frac{1}{2}$$ and $$x + 4 = 0$$ gives $$x = -4$$.  
   Solutions:  
   $$
   x = -\frac{1}{2}, \quad x = -4
   $$

### Medium

7. **Solve the quadratic equation $$6x^2 + 13x + 6 = 0$$ by factoring by grouping:**  
   **Step 1:** The equation is already in standard form.  
   **Step 2:** Multiply $$a$$ and $$c$$: $$6 \times 6 = 36$$.  
   **Step 3:** Find two numbers that multiply to 36 and add to 13: $$9 \times 4 = 36$$ and $$9 + 4 = 13$$.  
   **Step 4:** Rewrite the middle term: $$6x^2 + 9x - 4x + 6 = 0$$.  
   **Step 5:** Group and factor: $$(6x^2 + 9x) - (4x + 6) = 0$$. Factor out the GCF: $$3x(2x + 3) - 2(2x + 3) = 0$$.  
   **Step 6:** Factor out the common binomial: $$(3x - 2)(2x + 3) = 0$$.  
   **Step 7:** Solve for $$x$$: $$3x - 2 = 0$$ gives $$x = \frac{2}{3}$$ and $$2x + 3 = 0$$ gives $$x = -\frac{3}{2}$$.  
   Solutions:  
   $$
   x = \frac{2}{3}, \quad x = -\frac{3}{2}
   $$

9. **Solve the quadratic equation $$5x^2 + 19x + 12 = 0$$ by factoring by grouping:**  
   **Step 1:** The equation is already in standard form.  
   **Step 2:** Multiply $$a$$ and $$c$$: $$5 \times 12 = 60$$.  
   **Step 3:** Find two numbers that multiply to 60 and add to 19: $$15 \times 4 = 60$$ and $$15 + 4 = 19$$.  
   **Step 4:** Rewrite the middle term: $$5x^2 + 15x + 4x + 12 = 0$$.  
   **Step 5:** Group and factor: $$(5x^2 + 15x) + (4x + 12) = 0$$. Factor out the GCF: $$5x(x + 3) + 4(x + 3) = 0$$.  
   **Step 6:** Factor out the common binomial: $$(5x + 4)(x + 3) = 0$$.  
   **Step 7:** Solve for $$x$$: $$5x + 4 = 0$$ gives $$x = -\frac{4}{5}$$ and $$x + 3 = 0$$ gives $$x = -3$$.  
   Solutions:  
   $$
   x = -\frac{4}{5}, \quad x = -3
   $$

11. **Solve the quadratic equation $$9x^2 + 18x + 4 = 0$$ by factoring by grouping:**  
   **Step 1:** The equation is already in standard form.  
   **Step 2:** Multiply $$a$$ and $$c$$: $$9 \times 4 = 36$$.  
   **Step 3:** Find two numbers that multiply to 36 and add to 18: $$12 \times 6 = 36$$ and $$12 + 6 = 18$$.  
   **Step 4:** Rewrite the middle term: $$9x^2 + 12x + 6x + 4 = 0$$.  
   **Step 5:** Group and factor: $$(9x^2 + 12x) + (6x + 4) = 0$$. Factor out the GCF: $$3x(3x + 4) + 2(3x + 4) = 0$$.  
   **Step 6:** Factor out the common binomial: $$(3x + 2)(3x + 4) = 0$$.  
   **Step 7:** Solve for $$x$$: $$3x + 2 = 0$$ gives $$x = -\frac{2}{3}$$ and $$3x + 4 = 0$$ gives $$x = -\frac{4}{3}$$.  
   Solutions:  
   $$
   x = -\frac{2}{3}, \quad x = -\frac{4}{3}
   $$

13. **Solve the quadratic equation $$7x^2 + 27x + 12 = 0$$ by factoring by grouping:**  
   **Step 1:** The equation is already in standard form.  
   **Step 2:** Multiply $$a$$ and $$c$$: $$7 \times 12 = 84$$.  
   **Step 3:** Find two numbers that multiply to 84 and add to 27: $$21 \times 4 = 84$$ and $$21 + 6 = 27$$.  
   **Step 4:** Rewrite the middle term: $$7x^2 + 21x + 6x + 12 = 0$$.  
   **Step 5:** Group and factor: $$(7x^2 + 21x) + (6x + 12) = 0$$. Factor out the GCF: $$7x(x + 3) + 2(3x + 6) = 0$$.  
   **Step 6:** Factor out the common binomial: $$(7x + 6)(x + 3) = 0$$.  
   **Step 7:** Solve for $$x$$: $$7x + 6 = 0$$ gives $$x = -\frac{6}{7}$$ and $$x + 3 = 0$$ gives $$x = -3$$.  
   Solutions:  
   $$
   x = -\frac{6}{7}, \quad x = -3
   $$

15. **Solve the quadratic equation $$8x^2 + 26x + 9 = 0$$ by factoring by grouping:**  
   **Step 1:** The equation is already in standard form.  
   **Step 2:** Multiply $$a$$ and $$c$$: $$8 \times 9 = 72$$.  
   **Step 3:** Find two numbers that multiply to 72 and add to 26: $$18 \times 4 = 72$$ and $$18 + 8 = 26$$.  
   **Step 4:** Rewrite the middle term: $$8x^2 + 18x + 8x + 9 = 0$$.  
   **Step 5:** Group and factor: $$(8x^2 + 18x) + (8x + 9) = 0$$. Factor out the GCF: $$2x(4x + 9) + 1(4x + 9) = 0$$.  
   **Step 6:** Factor out the common binomial: $$(2x + 1)(4x + 9) = 0$$.  
   **Step 7:** Solve for $$x$$: $$2x + 1 = 0$$ gives $$x = -\frac{1}{2}$$ and $$4x + 9 = 0$$ gives $$x = -\frac{9}{4}$$.  
   Solutions:  
   $$
   x = -\frac{1}{2}, \quad x = -\frac{9}{4}
   $$

17. **Solve the quadratic equation $$5x^2 + 16x + 3 = 0$$ by factoring by grouping:**  
   **Step 1:** The equation is already in standard form.  
   **Step 2:** Multiply $$a$$ and $$c$$: $$5 \times 3 = 15$$.  
   **Step 3:** Find two numbers that multiply to 15 and add to 16: $$15 \times 1 = 15$$ and $$15 + 1 = 16$$.  
   **Step 4:** Rewrite the middle term: $$5x^2 + 15x + x + 3 = 0$$.  
   **Step 5:** Group and factor: $$(5x^2 + 15x) + (x + 3) = 0$$. Factor out the GCF: $$5x(x + 3) + 1(x + 3) = 0$$.  
   **Step 6:** Factor out the common binomial: $$(5x + 1)(x + 3) = 0$$.  
   **Step 7:** Solve for $$x$$: $$5x + 1 = 0$$ gives $$x = -\frac{1}{5}$$ and $$x + 3 = 0$$ gives $$x = -3$$.  
   Solutions:  
   $$
   x = -\frac{1}{5}, \quad x = -3
   $$

### Hard

19. **Solve the quadratic equation $$12x^2 + 29x + 10 = 0$$ by factoring by grouping:**  
   **Step 1:** The equation is already in standard form.  
   **Step 2:** Multiply $$a$$ and $$c$$: $$12 \times 10 = 120$$.  
   **Step 3:** Find two numbers that multiply to 120 and add to 29: $$20 \times 6 = 120$$ and $$20 + 9 = 29$$.  
   **Step 4:** Rewrite the middle term: $$12x^2 + 20x + 9x + 10 = 0$$.  
   **Step 5:** Group and factor: $$(12x^2 + 20x) + (9x + 10) = 0$$. Factor out the GCF: $$4x(3x + 5) + 1(3x + 5) = 0$$.  
   **Step 6:** Factor out the common binomial: $$(4x + 1)(3x + 5) = 0$$.  
   **Step 7:** Solve for $$x$$: $$4x + 1 = 0$$ gives $$x = -\frac{1}{4}$$ and $$3x + 5 = 0$$ gives $$x = -\frac{5}{3}$$.  
   Solutions:  
   $$
   x = -\frac{1}{4}, \quad x = -\frac{5}{3}
   $$

21. **Solve the quadratic equation $$20x^2 + 39x + 18 = 0$$ by factoring by grouping:**  
   **Step 1:** The equation is already in standard form.  
   **Step 2:** Multiply $$a$$ and $$c$$: $$20 \times 18 = 360$$.  
   **Step 3:** Find two numbers that multiply to 360 and add to 39: $$30 \times 12 = 360$$ and $$30 + 9 = 39$$.  
   **Step 4:** Rewrite the middle term: $$20x^2 + 30x + 9x + 18 = 0$$.  
   **Step 5:** Group and factor: $$(20x^2 + 30x) + (9x + 18) = 0$$. Factor out the GCF: $$10x(2x + 3) + 3(2x + 6) = 0$$.  
   **Step 6:** Factor out the common binomial: $$(10x + 3)(2x + 6) = 0$$.  
   **Step 7:** Solve for $$x$$: $$10x + 3 = 0$$ gives $$x = -\frac{3}{10}$$ and $$2x + 6 = 0$$ gives $$x = -3$$.  
   Solutions:  
   
   $$
   x = -\frac{3}{10}, \quad x = -3
   $$