# Problem Set: Mathematics

## Table of Contents
1. [Factoring](#factoring)
2. [Trigonometric Ratios](#trigonometric-ratios)
3. [Additional Sections](#additional-sections)
4. [Additional Resources](#additional-resources)

---

## Instructions
- **Attempt Each Problem First**: Try to solve each problem on your own before revealing the solution.
- **View Solutions**: Click on the "Solution" button below each problem to see the detailed answer.

---

## I. Factoring
**Factor the quadratic equation:**

1. $x^2 - 5x + 6 = 0$

    <details>
        <summary><strong>ðŸ”Ž Hint</strong></summary>

    To factor the quadratic equation, look for two numbers that multiply to **+6** and add up to **-5**.
    </details>

    <details>
        <summary><strong>ðŸ’¡ Answer</strong></summary>

    $(x - 2)(x - 3) = 0$
    </details>

    <details>
        <summary><strong>ðŸ”“ Solution</strong></summary>

    **Step 1:** Identify two numbers that multiply to **+6** (the constant term) and add up to **-5** (the coefficient of the middle term).
    
    **Step 2:** The numbers **-2** and **-3** satisfy these conditions since:
    
    $-2 \times -3 = 6$

    $-2 + (-3) = -5$
    
    **Step 3:** Rewrite the quadratic equation using these numbers:
    
    $x^2 - 2x - 3x + 6 = 0$
    
    **Step 4:** Factor by grouping:

    $x(x - 2) - 3(x - 2) = 0$

    **Step 5:** Factor out the common term $(x - 2)$:
    
    $(x - 3)(x - 2) = 0$
    </details>

2. $2x^2 + 7x + 3 = 0$

    <details>
        <summary><strong>ðŸ”Ž Hint</strong></summary>

        Look for two numbers that multiply to **2 Ã— 3 = 6** and add up to **+7**.
    </details>

    <details>
        <summary><strong>ðŸ’¡ Answer</strong></summary>

        $(2x + 1)(x + 3) = 0$
    </details>

    <details>
        <summary><strong>ðŸ”“ Solution</strong></summary>

        **Step 1:** Multiply the leading coefficient and the constant term: \( 2 Ã— 3 = 6 \).

        **Step 2:** Find two numbers that multiply to **+6** and add up to **+7**. The numbers **+6** and **+1** satisfy these conditions:
        $$
        6 Ã— 1 = 6 \\
        6 + 1 = 7
        $$

        **Step 3:** Rewrite the middle term using these numbers:
        $$
        2x^2 + 6x + x + 3 = 0
        $$

        **Step 4:** Factor by grouping:
        $$
        2x(x + 3) + 1(x + 3) = 0
        $$

        **Step 5:** Factor out the common binomial \((x + 3)\):
        $$
        (2x + 1)(x + 3) = 0
        $$

        **Conclusion:** The factored form is \( (2x + 1)(x + 3) = 0 \).
    </details>

3. $x^2 - 9 = 0$

    <details>
        <summary><strong>ðŸ”Ž Hint</strong></summary>

        Recognize that this is a **difference of squares**.
    </details>

    <details>
        <summary><strong>ðŸ’¡ Answer</strong></summary>

        $(x - 3)(x + 3) = 0$
    </details>

    <details>
        <summary><strong>ðŸ”“ Solution</strong></summary>

        **Step 1:** Identify the expression as a difference of squares:
        $$
        x^2 - 9 = x^2 - 3^2
        $$

        **Step 2:** Apply the difference of squares formula \( a^2 - b^2 = (a - b)(a + b) \):
        $$
        (x - 3)(x + 3) = 0
        $$

        **Conclusion:** The factored form is \( (x - 3)(x + 3) = 0 \).
    </details>

4. $3x^2 - 12x + 12 = 0$

    <details>
        <summary><strong>ðŸ”Ž Hint</strong></summary>

        Factor out the greatest common factor (GCF) before proceeding.
    </details>

    <details>
        <summary><strong>ðŸ’¡ Answer</strong></summary>

        $3(x - 2)^2 = 0$
    </details>

    <details>
        <summary><strong>ðŸ”“ Solution</strong></summary>

        **Step 1:** Factor out the GCF, which is **3**:
        $$
        3x^2 - 12x + 12 = 3(x^2 - 4x + 4)
        $$

        **Step 2:** Factor the quadratic expression inside the parentheses:
        $$
        x^2 - 4x + 4 = (x - 2)^2
        $$

        **Step 3:** Substitute back:
        $$
        3(x - 2)^2 = 0
        $$

        **Conclusion:** The factored form is \( 3(x - 2)^2 = 0 \).
    </details>

---

5. $x^3 - 27 = 0$

    <details>
        <summary><strong>ðŸ”Ž Hint</strong></summary>

        Recognize this as a **difference of cubes**.
    </details>

    <details>
        <summary><strong>ðŸ’¡ Answer</strong></summary>

        $(x - 3)(x^2 + 3x + 9) = 0$
    </details>

    <details>
        <summary><strong>ðŸ”“ Solution</strong></summary>

        **Step 1:** Identify the expression as a difference of cubes:
        $$
        x^3 - 27 = x^3 - 3^3
        $$

        **Step 2:** Apply the difference of cubes formula \( a^3 - b^3 = (a - b)(a^2 + ab + b^2) \):
        $$
        (x - 3)(x^2 + 3x + 9) = 0
        $$

        **Conclusion:** The factored form is \( (x - 3)(x^2 + 3x + 9) = 0 \).
    </details>

---

6. $4x^2 - 12x + 9 = 0$

    <details>
        <summary><strong>ðŸ”Ž Hint</strong></summary>

        Check if the quadratic is a **perfect square trinomial**.
    </details>

    <details>
        <summary><strong>ðŸ’¡ Answer</strong></summary>

        $(2x - 3)^2 = 0$
    </details>

    <details>
        <summary><strong>ðŸ”“ Solution</strong></summary>

        **Step 1:** Determine if the quadratic is a perfect square trinomial by checking if:
        - The first term is a perfect square: \( (2x)^2 = 4x^2 \).
        - The last term is a perfect square: \( 3^2 = 9 \).
        - The middle term is twice the product of the square roots of the first and last terms: \( 2 Ã— 2x Ã— 3 = 12x \), which matches the middle term \( -12x \) with the appropriate sign.

        **Step 2:** Express the quadratic as a squared binomial:
        $$
        4x^2 - 12x + 9 = (2x - 3)^2
        $$

        **Conclusion:** The factored form is \( (2x - 3)^2 = 0 \).
    </details>

---

7. $x^4 - 16 = 0$

    <details>
        <summary><strong>ðŸ”Ž Hint</strong></summary>

        Notice that \( x^4 = (x^2)^2 \), making this a **difference of squares**.
    </details>

    <details>
        <summary><strong>ðŸ’¡ Answer</strong></summary>

        $(x^2 - 4)(x^2 + 4) = 0$
    </details>

    <details>
        <summary><strong>ðŸ”“ Solution</strong></summary>

        **Step 1:** Rewrite \( x^4 - 16 \) as a difference of squares:
        $$
        x^4 - 16 = (x^2)^2 - 4^2
        $$

        **Step 2:** Apply the difference of squares formula \( a^2 - b^2 = (a - b)(a + b) \):
        $$
        (x^2 - 4)(x^2 + 4) = 0
        $$

        **Step 3:** Factor further if possible. Notice that \( x^2 - 4 \) is also a difference of squares:
        $$
        x^2 - 4 = (x - 2)(x + 2)
        $$

        **Step 4:** Combine the factors:
        $$
        (x - 2)(x + 2)(x^2 + 4) = 0
        $$

        **Conclusion:** The fully factored form is \( (x - 2)(x + 2)(x^2 + 4) = 0 \).
    </details>

---

8. $6x^3 - 15x^2 + 6x = 0$

    <details>
        <summary><strong>ðŸ”Ž Hint</strong></summary>

        Factor out the greatest common factor (GCF) first.
    </details>

    <details>
        <summary><strong>ðŸ’¡ Answer</strong></summary>

        $3x(2x^2 - 5x + 2) = 0$
    </details>

    <details>
        <summary><strong>ðŸ”“ Solution</strong></summary>

        **Step 1:** Identify and factor out the GCF, which is **3x**:
        $$
        6x^3 - 15x^2 + 6x = 3x(2x^2 - 5x + 2)
        $$

        **Step 2:** Factor the quadratic expression \( 2x^2 - 5x + 2 \):
        - Look for two numbers that multiply to **2 Ã— 2 = 4** and add up to **-5**. The numbers **-4** and **-1** satisfy this:
          $$
          -4 Ã— -1 = 4 \\
          -4 + (-1) = -5
          $$

        **Step 3:** Rewrite the quadratic using these numbers:
        $$
        2x^2 - 4x - x + 2 = 0
        $$

        **Step 4:** Factor by grouping:
        $$
        2x(x - 2) - 1(x - 2) = 0
        $$

        **Step 5:** Factor out the common term \((x - 2)\):
        $$
        (2x - 1)(x - 2) = 0
        $$

        **Conclusion:** The fully factored form is \( 3x(2x - 1)(x - 2) = 0 \).
    </details>

---

9. $x^2 + 5x + 6 = 0$

    <details>
        <summary><strong>ðŸ”Ž Hint</strong></summary>

        Find two numbers that multiply to **+6** and add up to **+5**.
    </details>

    <details>
        <summary><strong>ðŸ’¡ Answer</strong></summary>

        $(x + 2)(x + 3) = 0$
    </details>

    <details>
        <summary><strong>ðŸ”“ Solution</strong></summary>

        **Step 1:** Identify two numbers that multiply to **+6** and add up to **+5**. The numbers **+2** and **+3** satisfy these conditions:
        $$
        2 Ã— 3 = 6 \\
        2 + 3 = 5
        $$

        **Step 2:** Rewrite the quadratic equation using these numbers:
        $$
        x^2 + 2x + 3x + 6 = 0
        $$

        **Step 3:** Factor by grouping:
        $$
        x(x + 2) + 3(x + 2) = 0
        $$

        **Step 4:** Factor out the common term \((x + 2)\):
        $$
        (x + 2)(x + 3) = 0
        $$

        **Conclusion:** The factored form is \( (x + 2)(x + 3) = 0 \).
    </details>

---

10. $x^2 - 4x - 5 = 0$

    <details>
        <summary><strong>ðŸ”Ž Hint</strong></summary>

        Find two numbers that multiply to **-5** and add up to **-4**.
    </details>

    <details>
        <summary><strong>ðŸ’¡ Answer</strong></summary>

        $(x - 5)(x + 1) = 0$
    </details>

    <details>
        <summary><strong>ðŸ”“ Solution</strong></summary>

        **Step 1:** Identify two numbers that multiply to **-5** and add up to **-4**. The numbers **-5** and **+1** satisfy these conditions:
        $$
        -5 Ã— 1 = -5 \\
        -5 + 1 = -4
        $$

        **Step 2:** Rewrite the quadratic equation using these numbers:
        $$
        x^2 - 5x + x - 5 = 0
        $$

        **Step 3:** Factor by grouping:
        $$
        x(x - 5) + 1(x - 5) = 0
        $$

        **Step 4:** Factor out the common term \((x - 5)\):
        $$
        (x - 5)(x + 1) = 0
        $$

        **Conclusion:** The factored form is \( (x - 5)(x + 1) = 0 \).
    </details>

---

11. $x^3 - 3x^2 - 4x + 12 = 0$

    <details>
        <summary><strong>ðŸ”Ž Hint</strong></summary>

        Use the Rational Root Theorem to find a root, then factor by grouping.
    </details>

    <details>
        <summary><strong>ðŸ’¡ Answer</strong></summary>

        $(x - 3)(x + 2)(x - 2) = 0$
    </details>

    <details>
        <summary><strong>ðŸ”“ Solution</strong></summary>

        **Step 1:** Apply the Rational Root Theorem to identify possible rational roots. The possible roots are \( \pm1, \pm2, \pm3, \pm4, \pm6, \pm12 \).

        **Step 2:** Test \( x = 3 \):
        $$
        3^3 - 3(3)^2 - 4(3) + 12 = 27 - 27 - 12 + 12 = 0
        $$
        Thus, \( x = 3 \) is a root.

        **Step 3:** Perform polynomial division or synthetic division to factor out \( (x - 3) \):
        $$
        x^3 - 3x^2 - 4x + 12 = (x - 3)(x^2 + 0x - 4)
        $$

        **Step 4:** Factor the quadratic \( x^2 - 4 \):
        $$
        x^2 - 4 = (x - 2)(x + 2)
        $$

        **Step 5:** Combine the factors:
        $$
        (x - 3)(x - 2)(x + 2) = 0
        $$

        **Conclusion:** The fully factored form is \( (x - 3)(x + 2)(x - 2) = 0 \).
    </details>

---

### Problem 2
**Simplify the expression:**
$$
\frac{\tan(\theta)}{1 + \cot(\theta)}
$$

<details>
  <summary><strong>Solution</strong></summary>
  
Start by expressing \( \tan(\theta) \) and \( \cot(\theta) \) in terms of sine and cosine:
$$
\tan(\theta) = \frac{\sin(\theta)}{\cos(\theta)} \\
\cot(\theta) = \frac{\cos(\theta)}{\sin(\theta)}
$$

Substitute into the original expression:
$$
\frac{\frac{\sin(\theta)}{\cos(\theta)}}{1 + \frac{\cos(\theta)}{\sin(\theta)}} = \frac{\sin(\theta)}{\cos(\theta)} \div \left( \frac{\sin(\theta) + \cos(\theta)}{\sin(\theta)} \right) = \frac{\sin^2(\theta)}{\cos(\theta)(\sin(\theta) + \cos(\theta))}
$$

Simplify by factoring:
$$
\frac{\sin(\theta)}{\cos(\theta)} \cdot \frac{\sin(\theta)}{\sin(\theta) + \cos(\theta)} = \tan(\theta) \cdot \frac{\sin(\theta)}{\sin(\theta) + \cos(\theta)}
$$

Final simplified form:
$$
\frac{\sin^2(\theta)}{\cos(\theta)(\sin(\theta) + \cos(\theta))}
$$

</details>

---

### Problem 3
**Prove that \( \tan(\theta) + \cot(\theta) = \frac{2}{\sin(2\theta)} \).**

<details>
  <summary><strong>Solution</strong></summary>
  
Start with the left-hand side (LHS):
$$
\tan(\theta) + \cot(\theta) = \frac{\sin(\theta)}{\cos(\theta)} + \frac{\cos(\theta)}{\sin(\theta)} = \frac{\sin^2(\theta) + \cos^2(\theta)}{\sin(\theta)\cos(\theta)} = \frac{1}{\sin(\theta)\cos(\theta)}
$$

Recall the double-angle identity for sine:
$$
\sin(2\theta) = 2\sin(\theta)\cos(\theta) \quad \Rightarrow \quad \sin(\theta)\cos(\theta) = \frac{\sin(2\theta)}{2}
$$

Substitute into the LHS:
$$
\frac{1}{\sin(\theta)\cos(\theta)} = \frac{2}{\sin(2\theta)}
$$

Therefore:
$$
\tan(\theta) + \cot(\theta) = \frac{2}{\sin(2\theta)}
$$

</details>

---

## Additional Sections

> **Note:** This section is a placeholder. You can add more sections for different types of problems following the structure used in the "Factoring" and "Trigonometric Ratios" sections.

### Section Title
**Description:**
Brief description of the problem type.

### Problem X
**Description:**
Detailed problem statement.

<details>
  <summary><strong>Solution</strong></summary>
  
Detailed solution steps, including any necessary LaTeX expressions.

</details>

---

## Additional Resources
- [Markdown Guide](https://www.markdownguide.org/)
- [GitHub Flavored Markdown Spec](https://github.github.com/gfm/)
- [LaTeX Project](https://www.latex-project.org/)
- [Wolfram MathWorld](https://mathworld.wolfram.com/)

---

## Notes
- **LaTeX Rendering:** Ensure that LaTeX expressions are correctly formatted. Use `$$ ... $$` for display math and `$ ... $` for inline math.
- **Table of Contents:** Update the Table of Contents as you add new sections to maintain easy navigation.
- **Consistent Formatting:** Maintain a uniform structure for each problem and solution to ensure readability.
- **Expandability:** Easily add more sections and problems by following the established template structure.
- **Previewing:** Regularly push your Markdown file to GitHub and use the platform's preview feature to ensure everything renders correctly.

---